effect handler for unsupported_instruction can implement custom ISA extensions

Kraken/Examples/CustomInstructions.lean
@@ -1,20 +1,86 @@
 import Kraken.Semantics
 import Kraken.Parser
 
+structure ExtraState where
+  bells: UInt64
+  whistles: UInt64
+  deriving Repr, BEq, DecidableEq, Hashable, Lean.ToExpr
+
+abbrev SystemState := MachineState × ExtraState
+
+-- Note: We do not get access to rip here.
+-- We also don't need it here, but other unsupported-instruction handlers might
+-- need it in order to jump to a handler implemented in assembly (rather
+-- than a handler modeled in Lean like here).
+def handle_bells_and_whistles (s : MachineData) (extra : ExtraState)
+  (i : Instr) (ok : MachineData → ExtraState → Except String SystemState)
+  : Except String SystemState :=
+  match i.operation with
+  | Operation.generic mnemonic operands =>
+    let mn := mnemonic.toLower
+    if mn = "rdbells" && operands = [] then
+      -- bells are always 64-bit, and rdbells' implicit dest is %rax
+      ok (s.setReg Reg.rax extra.bells.toBitVec) extra
+    else if mn.startsWith "rdwhistles" &&
+            mn.length = "rdwhistles_".length then
+      -- whistles are accessible as 8/16/32/64 bit
+      match operands with
+      | [.regOrMem (.reg r)] =>
+          ok (s.setReg r (extra.whistles.toBitVec.setWidth _)) extra
+      | _ => .error s!"wrong number of operands for rdwhistles"
+    else if mn = "wrbells" && operands = [] then
+      -- bells are always 64-bit, and wdbells' implicit source is %rax
+      ok s { extra with bells := s.regs.rax }
+    else if mn.startsWith "wrwhistles" &&
+            mn.length = "wrwhistles_".length then
+      -- whistles are accessible as 8/16/32/64 bit
+      match operands with
+      | [.regOrMem (.reg r)] =>
+        ok s { extra with whistles := UInt64.ofBitVec ((s.regs.get r).setWidth _) }
+      | _ => .error s!"wrong number of operands for wrwhistles"
+    else .error s!"unsupported instruction {repr i}"
+  | _ => .error s!"unsupported instruction {repr i}"
+
+def handle_effects (extra : ExtraState) (es : Effects)
+  (ok : SystemState → Except String SystemState)
+: Except String SystemState :=
+  match es with
+  | .done ms => ok (.mk ms extra)
+  | .undefined msg => .error msg
+  | .unimplemented msg => .error msg
+  | .unsupported_instruction s i resume =>
+       handle_bells_and_whistles s extra i (fun s' extra' =>
+         handle_effects extra' (resume s') ok)
+  | .can_read _ _ cont => handle_effects extra (cont true) ok
+  | .can_write _ _ cont => handle_effects extra (cont true) ok
+  | .can_exec _ cont => handle_effects extra (cont true) ok
+  | .nonmem_load addr .. => .error s!"Load at unmapped address {repr addr}"
+  | .nonmem_store addr .. => .error s!"Store at unmapped address {repr addr}"
+  | @Effects.pick _ t cont => handle_effects extra (cont (t.from_hash (hash extra))) ok
+
+partial def Executable.eval_with_bells_and_whistles (e : Executable)
+  (until_ : SystemState → Bool) (s : SystemState) : Except String SystemState :=
+  if until_ s then .ok s
+  else handle_effects s.2 (e.straightline s.1 .done)
+          (Executable.eval_with_bells_and_whistles e until_)
+
 def _start: String := "_start"
 def _end: String := "_end"
 
-def finishCriterion (p: Program) (s: MachineState): Bool :=
-  s.2 = p.fakeLayout.labels.label _end
+def finishCriterion (p: Program) (s: SystemState): Bool :=
+  s.1.2 = p.fakeLayout.labels.label _end
 
-def runKraken (asmCode : String) : Except String MachineState := do
+def runKraken (asmCode : String) : Except String SystemState := do
   let prog ← Kraken.Parser.parse_lenient (_start ++ ":" ++ asmCode ++ "\n" ++ _end ++ ":")
-  let initState: MachineState := ({dmem := ∅, regs := {
+  let initState: SystemState := (({dmem := ∅, regs := {
     rax := 42,
     rbx := 43,
     rcx := 44,
-  }}, prog.fakeLayout.labels.label _start)
-  prog.fakeLayout.eval initState (finishCriterion prog)
+  }}, prog.fakeLayout.labels.label _start), {
+    bells := 0xB3115,
+    whistles := 0x1141571E5,
+  })
+  prog.fakeLayout.eval_with_bells_and_whistles (finishCriterion prog) initState
 
 def simple_swap : String :=
  "mov %rax, %rcx
@@ -23,10 +89,8 @@ def simple_swap : String :=
 
 def run_and_get_rax_and_rbx (prog : String): UInt64 × UInt64 :=
   match runKraken prog with
-  | .ok s => (s.1.regs.rax, s.1.regs.rbx)
+  | .ok s => (s.1.1.regs.rax, s.1.1.regs.rbx)
   | .error _ => (-1, -1)
-
--- #eval Kraken.Parser.parse_lenient simple_swap
 
 example : run_and_get_rax_and_rbx simple_swap = (43, 42) := by native_decide
 
@@ -41,12 +105,14 @@ example : parse_or_nil "lol %eax, %ebx, $42" = [Directive.instr
      operation := .generic "lol" [Reg.eax, Reg.ebx, ConstExpr.int64 42] }] :=
   by native_decide
 
-def swap_bells_and_whistles_TODO_why_does_this_not_work : String :=
+def swap_bells_and_whistles_TODO_why_does_this_not_parse : String :=
  "rdbells            # bells are always 64-bit, and rdbells' implicit dest is %rax
   rdwhistlesl %ebx   # whistles are accessible as 8/16/32/64 bit, here we use the l suffix to get 32 bits
   wrwhistlesq %rax   # q suffix means we write 64 bits
   mov %rbx, %rax     # need to move to implicit argument register first
   wrbells            # always writes 64 bits from %rax"
+
+-- #eval runKraken swap_bells_and_whistles_TODO_why_does_this_not_parse
 
 def swap_bells_and_whistles : String :=
  "# bells are always 64-bit, and rdbells' implicit dest is %rax
@@ -60,17 +126,12 @@ def swap_bells_and_whistles : String :=
   # always writes 64 bits from %rax
   wrbells"
 
-def run_and_get_bells_and_whistles (prog : String): UInt64 × UInt64 :=
+def run_and_get_bells_and_whistles (prog : String): ExtraState :=
   match runKraken prog with
-  | .ok s => (s.1.regs.rax, s.1.regs.rbx)
-  | .error _ => (-1, -1)
+  | .ok s => s.2
+  | .error _ => { bells := -1, whistles := -1 }
 
-def run_and_get_error (prog : String): String :=
-  match runKraken prog with
-  | .ok _ => "actually, no error"
-  | .error msg => msg
-
--- #eval runKraken swap_bells_and_whistles
-
--- example : run_and_get_bells_and_whistles swap_bells_and_whistles = (43, 42) := by native_decide
-example : run_and_get_error swap_bells_and_whistles = "unsupported instruction { address_size := Width.W64, operation_size := Width.W64, operation := Operation.generic \"rdbells\" [] }" := by native_decide
+example : run_and_get_bells_and_whistles swap_bells_and_whistles = {
+   bells := 0x141571E5, -- rdwhistlesl only read 32 bits, so the first 1 got truncated!
+   whistles := 0xB3115
+} := by native_decide
